merge conflicts and rebase

theories/prob_eff_lang/probblaze/examples/DH_KE/sec_channel_prf.v
@@ -1,6 +1,7 @@
-From iris.proofmode Require Import base proofmode classes.
-From iris.base_logic.lib Require Import  na_invariants.
-From iris.algebra Require Import agree excl auth frac excl_auth.
+
+From iris.proofmode Require Import base proofmode classes.                                             
+From iris.base_logic.lib Require Import  na_invariants.   
+From iris.algebra Require Import agree excl auth frac excl_auth. 
 From iris.algebra.lib Require Import dfrac_agree.
 From clutch Require Import stdpp_ext.
 From clutch.prob_eff_lang.probblaze Require Import logic primitive_laws proofmode
@@ -33,7 +34,9 @@ Section schan_security.
   Variable xor_struct : XOR (Key := S (S n'')) (Support := S (S n'')).
   Context `{!XOR_spec (Key := S (S n'')) (Support := S (S n'')) (H := xor_struct)}.
   Variable group_xor_sem : vgG -> vgG -> vgG.
+  (* actual BITWISE xor has both left and right inverse, so this assumption is a valid spec.*)
   Hypothesis Bij_xor_sem : ∀ g1 g2 : vgG, group_xor_sem (group_xor_sem g1 g2) g2 = g1.
+  Hypothesis Bij_xor_sem_l : ∀ g1 g2 : vgG, group_xor_sem g1 (group_xor_sem g1 g2) = g2.
   Hypothesis vg_int_xor_sem : ∀ g1 g2 : vgG, vg_of_int_sem (xor_sem (int_of_vg_sem g1) (int_of_vg_sem g2)) = Some (group_xor_sem g1 g2 ).
   Variable log__g : vgG -> fin (S (S n'')).
   Hypothesis Val_log : ∀ x : vgG, (g ^+(log__g x))%g = x.
@@ -177,8 +180,10 @@ Section schan_security.
 
    (* semantic types*)
   (*----------------------------------------------------------------------------*)
-
-  Import valgroup_notation.
+    Definition sem_ty_group : sem_ty Σ := (λ v1 v2, ∃ g : vgG, ⌜ v1 = vgval g ⌝ ∗ ⌜ v2 = vgval g ⌝)%I.
+ 
+  Notation "'𝔾'" := sem_ty_group.
+ (* Import valgroup_notation.*)
 
   Program Definition keyleak_mono (keyleak1 keyleak2 : label) := {| pmono_prot_car := iThySum (iThySum (KLeakSendAlice keyleak1 keyleak2) (KLeakRecvAlice keyleak1 keyleak2)) (iThySum (KLeakSendBob keyleak1 keyleak2) (KLeakRecvBob keyleak1 keyleak2)) ; pmono_prot_prop := _|}.
   Next Obligation.
@@ -193,7 +198,8 @@ Section schan_security.
   Proof.
          intros. unfold pers_mono_row. iIntros (????) "#HΦΦ'". iIntros (???) "(%H1 & H2)".
          iSplitR "H2"; [iPureIntro; apply H1 |].
-         unfold keyleak in H1. simpl in H1. unfold keyleak_mono in H1. simpl in H1.       Search "∈". apply list_elem_of_singleton in H1. simpl in H1.
+         unfold keyleak in H1. simpl in H1. unfold keyleak_mono in H1. simpl in H1.
+         apply list_elem_of_singleton in H1. simpl in H1.
          inversion H1. simpl in *.
          iDestruct "H2" as (?e1' ?e2' ?k1 ?k2 ?S) "H2e1e2".
          iExists e1', e2', k1, k2, S.
@@ -255,7 +261,23 @@ Qed.
   Proof.
     intros. unfold pers_mono_row. iIntros (????) "#HΦΦ'". iIntros (???) "(%H1 & H2)".
          iSplitR "H2"; [iPureIntro; apply H1 |].
-         unfold keyleak in H1. simpl in H1. unfold keyleak_mono in H1. simpl in H1.       Search "∈". apply list_elem_of_singleton in H1. simpl in H1.
+         unfold keyleak in H1. simpl in H1. unfold keyleak_mono in H1. simpl in H1. apply list_elem_of_singleton in H1. simpl in H1.
+         inversion H1. simpl in *.
+         iDestruct "H2" as (?e1' ?e2' ?k1 ?k2 ?S) "H2e1e2".
+         iExists e1', e2', k1, k2, S.
+         iDestruct "H2e1e2" as "(%Hv1 & (%HNk1 & (%Hv2 & (%HNk2 & HS))))".
+         repeat iSplit; try iPureIntro; try auto.
+         { iDestruct "HS" as "(He1e2 & Hs1s2)". iApply "He1e2". }
+         { iDestruct "HS" as "(He1e2 & #Hs1s2)". iModIntro.
+           iIntros (??) "HS". iApply "HΦΦ'". iApply "Hs1s2". iApply "HS".
+         }
+  Qed.
+
+   Lemma client_pers_mono_row' (channel leaksec getKey1 schannel1 schannel2 : label) : ⊢ pers_mono_row (iLblSig_to_iLblThy [([leaksec; schannel1] , [channel; getKey1; schannel2] , sec_channel schannel1 schannel2)]).
+  Proof.
+    intros. unfold pers_mono_row. iIntros (????) "#HΦΦ'". iIntros (???) "(%H1 & H2)".
+         iSplitR "H2"; [iPureIntro; apply H1 |].
+         unfold keyleak in H1. simpl in H1. unfold keyleak_mono in H1. simpl in H1. apply list_elem_of_singleton in H1. simpl in H1.
          inversion H1. simpl in *.
          iDestruct "H2" as (?e1' ?e2' ?k1 ?k2 ?S) "H2e1e2".
          iExists e1', e2', k1, k2, S.
@@ -284,8 +306,10 @@ Qed.
 Qed.
 
   Program Definition sec_channel_row (schannel1 schannel2 : label) := SemRow [([schannel1], [schannel2], sec_channel schannel1 schannel2)] (sec_channel_pers_mono_row schannel1 schannel2).
-  Program Definition client_row (channel leaksec getKey1 schannel1 schannel2 : label) := SemRow [([channel; getKey1; schannel1], [leaksec; schannel2], sec_channel schannel1 schannel2)] (client_pers_mono_row channel leaksec getKey1 schannel1 schannel2) .
+  Program Definition client_row (channel leaksec getKey1 schannel1 schannel2 : label) := SemRow [([channel; getKey1; schannel1], [leaksec; schannel2], sec_channel schannel1 schannel2)] (client_pers_mono_row channel leaksec getKey1 schannel1 schannel2).
 
+  Program Definition client_row' (channel leaksec getKey1 schannel1 schannel2 : label) := SemRow [([leaksec; schannel1], [channel; getKey1; schannel2], sec_channel schannel1 schannel2)] (client_pers_mono_row' channel leaksec getKey1 schannel1 schannel2).
+  
    Definition REAL_CHAN : val :=
     λ: "f",
       (F_OAUTH ||ₗ F_KE_lazy_alice) (CHAN xor "f").
@@ -361,67 +385,43 @@ Qed.
    { simpl. iApply "Hrelxor". }
   Qed.
 
+
+   Lemma G_XOR_CORRECT_r (g1 g2 : vgG) E K X e R :
+    let g := (group_xor_sem g1 g2) in
+    (* vg_of_int_sem (xor_sem (int_of_vg_sem g1) (int_of_vg_sem g2)) = Some g1 ->*)
+     vg_of_int_sem (xor_sem (int_of_vg_sem g1) (int_of_vg_sem g2)) = Some g ->
+        (BREL e ≤ (fill K (SOMEV (vgval g))) @ E <|X|> {{R}}) -∗ 
+     (BREL e ≤ (fill K (G_XOR xor (vgval g1) (vgval g2))) @ E <|X|> {{R}}).
+  Proof using Bdd_int_vg G H XOR_spec0 group_xor_sem cg vg vgg xor_struct
+Σ.
+    simpl.
+    intro Hg1g2.
+    iIntros "Hrelxor".
+    unfold G_XOR.
+    brel_pures. 
+   assert (fill (K ++  [AppRCtx vg_of_int  ; AppRCtx (App xor (int_of_vg (vgval g1)))]) (int_of_vg (vgval g2)) = fill K (fill [AppRCtx vg_of_int  ; AppRCtx (App xor (int_of_vg (vgval g1)))] (int_of_vg (vgval g2)))) as Hectxappg2.
+   { rewrite fill_app. auto. }
+   rewrite -Hectxappg2.
+   iApply (brel_int_of_vg_sem_correct_r _ _ g2).
+   simpl.
+   rewrite fill_app. simpl.
+   assert (fill (K ++  [AppRCtx vg_of_int  ; AppLCtx #(int_of_vg_sem g2); AppRCtx xor]) (int_of_vg (vgval g1)) = fill K (fill [AppRCtx vg_of_int  ; AppLCtx #(int_of_vg_sem g2); AppRCtx xor] (int_of_vg (vgval g1)))) as Hectxappg1.
+   { rewrite fill_app. auto. }
+   rewrite -Hectxappg1.
+   iApply (brel_int_of_vg_sem_correct_r _ _ g1).
+   rewrite fill_app. simpl.
+   assert (fill (K ++ [AppRCtx vg_of_int ]) (xor #(int_of_vg_sem g1) #(int_of_vg_sem g2)) = fill K (fill [AppRCtx vg_of_int] (xor #(int_of_vg_sem g1) #(int_of_vg_sem g2)))) as Hectxxor.
+   { rewrite fill_app. auto. }
+   rewrite -Hectxxor.
+   iApply xor_correct_r; try (eapply Bdd_int_vg).
+   rewrite fill_app. simpl.
+   iApply brel_vg_of_int_correct_r.
+   { apply Hg1g2. }
+   { simpl. iApply "Hrelxor". }
+  Qed.
+
 (*secure channel only assumes a fixed direction of messag epassing, so this needs to relfect in the type of the thunks that its client receives*)
-(*Verification of F_OAUTH[F_KE_L[CHAN[]]] ≤ CHAN_SIM[F_CHAN[]]*)
-(*----------------------------------------------------------*)
-Lemma F_KE_CHAN_SIM (f1 f2 : val) (L : sem_row Σ) :
- (*(∀ᵣ θₕ, (((𝔾 × 𝟙 + 𝟙) -{ θₕ }-> 𝟙) × 𝟙 + 𝟙 -{ θₕ }-> Option 𝔾) -{ sem_row_union θₕ L }-∘ 𝟙)%T
-                 f1 f2 -∗*)
-   (∀ᵣ θₕ, (((𝔾 -{ θₕ }-> 𝟙) × (𝟙 -{ θₕ }-> Option 𝔾)) -{ sem_row_union θₕ L }-∘ 𝟙))%T
-                 f1 f2 -∗
-    BREL REAL_CHAN f1
-      ≤ CHAN_SIM_lazy (F_CHAN f2) <|⊥|> {{λ v1 v2,
-                                       ∀ (leakauth1 leakauth2 keyleak1 keyleak2 : label),
-                                       BREL v1 ((λ: "m", do: leakauth1 (Send "m")), (λ: "m", do: leakauth1 (Recv "m")))%V ((λ: "m", do: keyleak1 (Send "m")), (λ: "m", do: keyleak1 (Recv "m")))%V ≤ v2 ((λ: "m", do: leakauth2 (Send "m")), (λ: "m", do: leakauth2 (Recv "m")))%V ((λ: "m", do: keyleak2 (Send "m")), (λ: "m", do: keyleak2 (Recv "m")))%V <| (iLblSig_to_iLblThy (envsec_row keyleak1 keyleak2 leakauth1 leakauth2 )) ++ (iLblSig_to_iLblThy L) |> {{ (λ w1 w2, 𝟙%T w1 w2)}}}}.
-Proof with (repeat foldkont) using G H cg inG0 inG1 inG2 klk1 klk2 lka1 lka2 vg vgg Σ.
-Admitted.
 
-(*refinement in terms of semantic types for REAL_CHAN ≤ CHAN_SIM (F_CHAN) *)
-(*-------------------------------------------------------------------*)
-
-Lemma SEM_F_KE_CHAN_SIM (f1 f2 : val) (L : sem_row Σ) :
-    (∀ᵣ θₕ, ((𝔾 -{ θₕ }-> 𝟙) × (𝟙 -{ θₕ }-> Option 𝔾)) -{ sem_row_union θₕ L }-∘ 𝟙)%T
-                 f1 f2 -∗
-    BREL REAL_CHAN f1
-      ≤ CHAN_SIM_lazy (F_CHAN f2) <|⊥|> {{λ v1 v2,
-                                       (∀ᵣ θ₁, ∀ᵣ θ₂,  (((𝔾 × (𝟙 + 𝟙)) -{ θ₁ }-> 𝟙) × ((𝟙 + 𝟙) -{ θ₁ }-> Option 𝟙)) ⊸ ((((𝟙 + 𝟙) -{ θ₂ }-> 𝟙) × ((𝟙 + 𝟙) -{ θ₂ }-> Option 𝟙)) -{ sem_row_union (sem_row_union θ₁ θ₂) L }-∘ 𝟙))%T v1 v2 }}.
-Proof with (repeat foldkont) using G.
-Admitted.
-
-Lemma REAL_CHAN_CHAN_SIM_F_CHAN :
-  ⊢ sem_val_typed (REAL_CHAN)%V (λ: "f", CHAN_SIM_lazy (F_CHAN "f"))%V                                                                                         (∀ᵣ θ__L ,(∀ᵣ θₕ, (((𝔾 -{ θₕ }->  𝟙) × (𝟙 -{ θₕ }-> (Option 𝔾))) -{ sem_row_union  θₕ θ__L }-∘ 𝟙)) ⊸ (*type of client*)
-      (∀ᵣ θ₁, ∀ᵣ θ₂,  (((𝔾 × (𝟙 + 𝟙)) -{ θ₁ }-> 𝟙) × ((𝟙 + 𝟙) -{ θ₁ }-> Option 𝟙)) ⊸ (((𝟙 + 𝟙) -{ θ₂ }-> 𝟙) × (𝟙 + 𝟙) -{ θ₂ }-> Option 𝟙) -{ sem_row_union (sem_row_union θ₁ θ₂) θ__L }-∘ 𝟙))%T.
-Proof using G inG0 inG1 inG2.
-  iModIntro. iIntros (L).
-  iIntros (f1 f2) "Hrelf1f2".
-  brel_pures'.
-  simpl.
-  assert (to_iThyIfMono OS [] = []) as <- by done.
-  iApply (brel_mono OS with "[][Hrelf1f2]");
-  [iApply to_iThy_le_refl|simpl|simpl].
-  +  iApply (SEM_F_KE_CHAN_SIM _ _ L).
-     iApply "Hrelf1f2".
-  + iIntros (??) "$".
-Qed.
-
-(*top level statements for the secure channel *)
-(*----------------------------------------------------------------*)
-Lemma REAL_IDEAL_SCHAN :
-  ⊢ sem_typed [] REAL_CHAN (λ: "f", (CHAN_SIM_lazy (F_CHAN "f")))%V ⊥
-       (∀ᵣ θ__L ,(∀ᵣ θₕ, ((𝔾 -{ θₕ }-> 𝟙) × ( 𝟙 -{ θₕ }-> (Option  𝔾))) -{ sem_row_union  θₕ θ__L }-∘ 𝟙)%T ⊸ (*type of client*)
-                 (∀ᵣ θ₁, ∀ᵣ θ₂,  (((𝔾 × (𝟙 + 𝟙)) -{ θ₁ }-> 𝟙) × ((𝟙 + 𝟙) -{ θ₁ }-> Option 𝟙)) ⊸ (((𝟙 + 𝟙) -{ θ₂ }-> 𝟙) × ((𝟙 + 𝟙) -{ θ₂ }-> Option 𝟙)) -{ sem_row_union (sem_row_union θ₁ θ₂) θ__L }-∘ 𝟙))%T [].
-Proof using G inG0 inG1 inG2 klk1 klk2 lka1 lka2.
-  iIntros (vs) "!# H". simpl.
-  iApply brel_value.
-  iIntros "$ !>".
-  iSplit; try (done).
-  iPoseProof REAL_CHAN_CHAN_SIM_F_CHAN as "Hsemty".
-  rewrite /sem_val_typed /=.
-  iDestruct "Hsemty" as "#Hsemty".
-  iApply "Hsemty".
-Qed.
-
-(*Lemma IDEAl_REAL_SCHAN :*)
 
 Definition R_CHAN : val :=
    λ: "f",
@@ -436,7 +436,7 @@ Lemma F_OAUTH_CHAN_SIM (f1 f2 : val) (L : sem_row Σ) :
       ≤ CHAN_SIM_lazy (F_CHAN f2) <|⊥|> {{λ v1 v2,
                                        ∀ (leakauth1 leakauth2 keyleak1 keyleak2 : label),
                                        BREL v1 ((λ: "m", do: leakauth1 (Send "m")), (λ: "m", do: leakauth1 (Recv "m")))%V ((λ: "m", do: keyleak1 (Send "m")), (λ: "m", do: keyleak1 (Recv "m")))%V ≤ v2 ((λ: "m", do: leakauth2 (Send "m")), (λ: "m", do: leakauth2 (Recv "m")))%V ((λ: "m", do: keyleak2 (Send "m")), (λ: "m", do: keyleak2 (Recv "m")))%V  <| (iLblSig_to_iLblThy (envsec_row keyleak1 keyleak2 leakauth1 leakauth2 )) ++ (iLblSig_to_iLblThy L) |> {{ (λ w1 w2, 𝟙%T w1 w2)}}}}.
-Proof with (repeat foldkont) using Bdd_int_vg Bij_log Bij_xor_sem G
+Proof with (repeat foldkont) using Bdd_int_vg Bij_log Bij_xor_sem Bij_xor_sem_l G
 H Val_log XOR_spec0 cg group_xor_sem inG0
 inG1 inG2 klk1 klk2 lka1 lka2 log__g vg
 vg_int_xor_sem vgg xor_struct Σ.
@@ -449,19 +449,16 @@ vg_int_xor_sem vgg xor_struct Σ.
   unfold CHAN.
   repeat simpl. brel_pures'.
 
-  (*iApply (xor_correct_l ⊤ _ _ _ (CHAN_SIM (F_CHAN f2)) ⊥ _).*)
+  
   unfold F_CHAN, CHAN_SIM_lazy, F_KE_lazy_alice, F_OAUTH.
 
 
   repeat simpl. brel_pures. iModIntro. iIntros (????).
   brel_pures.
-  (*iApply brel_alloctape_r. iIntros (α) "Hα". brel_pures_r.*)
+
   iApply brel_alloc_r. iIntros (l_sim) "Hl_sim". brel_pures_r.
   iApply brel_alloc_r. iIntros (l_m'sim) "Hl_m'sim". brel_pures_r.
-  (*iApply brel_couple_UT. 1: auto.
-  simpl. iFrame "Hα". iSplit => //.
-  iIntros (n ?) "!> Hα". brel_pures.
-  brel_exp_l. brel_pures. *)
+ 
   iApply brel_alloctape_l. iIntros (γ) "!> Hγ". brel_pures_l.
   iApply brel_alloc_l. iIntros (l_key) "!> Hl_key". brel_pures_l.
    iApply brel_effect_l. iIntros (getKey') "!> HgK !>". brel_pures_l.
@@ -896,7 +893,8 @@ vg_int_xor_sem vgg xor_struct Σ.
            { iApply "Hrel". iApply "HmQ". }
            { iApply "IH". }
         ++ unfold d3.
-           iDestruct "Hd3" as (?m ?n) "(Hγ & (Hl_m'sim & (Hl_sim & (Hl_auth & (Hl_fchan & (Hl_rchan & Hl_key))))))".                iApply (brel_load_l _ _ _  [HandleCtx _ _ _ _ _ ; HandleCtx _ _ _ _ _ ; CaseCtx _ _] with "Hl_rchan").
+           iDestruct "Hd3" as (?m ?n) "(Hγ & (Hl_m'sim & (Hl_sim & (Hl_auth & (Hl_fchan & (Hl_rchan & Hl_key))))))".               
+           iApply (brel_load_l _ _ _  [HandleCtx _ _ _ _ _ ; HandleCtx _ _ _ _ _ ; CaseCtx _ _] with "Hl_rchan").
            iIntros "!> Hl_rchan'".
            brel_pures.
            iApply (brel_load_r _ _ _ _  [HandleCtx _ _ _ _ _ ; CaseCtx _ _] with "Hl_fchan").
@@ -1213,8 +1211,8 @@ Lemma SEM_R_CHAN_SIM (f1 f2 : val) (L : sem_row Σ) :
                  f1 f2 -∗
     BREL R_CHAN f1
       ≤ CHAN_SIM_lazy (F_CHAN f2) <|⊥|> {{λ v1 v2,
-                                       (∀ᵣ θ₁, ∀ᵣ θ₂,  (((𝔾 × (𝟙 + 𝟙)) -{ θ₁ }-> 𝟙) × ((𝟙 + 𝟙) -{ θ₁ }-> Option 𝟙)) ⊸ (((𝟙 + 𝟙) -{ θ₂ }-> 𝟙) ×(𝟙 + 𝟙) -{ θ₂ }-> Option 𝟙) -{ sem_row_union θ₁ (sem_row_union θ₂ L) }-∘ 𝟙)%T v1 v2 }}.
-Proof with (repeat foldkont) using  Bdd_int_vg Bij_log Bij_xor_sem G H
+                                       (∀ᵣ θ₁, ∀ᵣ θ₂,  (((𝔾 × (𝟙 + 𝟙)) -{ θ₁ }-> 𝟙) × ((𝟙 + 𝟙) -{ θ₁ }-> Option 𝟙)) ⊸ (((𝟙 + 𝟙) -{ θ₂ }-> 𝟙) ×(𝟙 + 𝟙) -{ θ₂ }-> Option 𝟙) -{ sem_row_union θ₁ (sem_row_union θ₂ L) }-∘ 𝟙)%T v1 v2 }}. 
+Proof with (repeat foldkont) using  Bdd_int_vg Bij_log Bij_xor_sem Bij_xor_sem_l G H
 Val_log XOR_spec0 cg group_xor_sem log__g vg
 vg_int_xor_sem vgg xor_struct Σ.
 
@@ -2064,15 +2062,938 @@ Qed.
 
 
 Lemma SEM_R_CHAN_SIM_rev (f1 f2 : val) (L : sem_row Σ) :
-  (* sem_val_typed f1 f2 ((∀ᵣ θₕ, (((⊤ × (sem_ty_sum 𝟙 𝟙)) -{ θₕ }-> (Option ⊤)) × ((sem_ty_sum 𝟙 𝟙) -{ θₕ }-> (Option ⊤))) -{ sem_row_union  θₕ L }-∘ 𝟙))%T -∗*)
    (∀ᵣ θₕ, (((𝔾 -{ θₕ }-> 𝟙) × (𝟙 -{ θₕ }-> Option 𝔾)) -{ sem_row_union θₕ L }-∘ 𝟙))%T
                  f1 f2 -∗
     BREL CHAN_SIM_lazy (F_CHAN f1)
       ≤ (R_CHAN f2) <|⊥|> {{λ v1 v2,
-                                       (* (∀ᵣ θ₁,  (((⊤ × (𝟙 + 𝟙)) -{ θ₁ }-> 𝟙) × ((𝟙 + 𝟙) -{ θ₁ }-> Option ⊤)) ⊸ ((𝟙 + 𝟙) -{ θ₁ }-> Option ⊤) -{ sem_row_union θ₁ L }-∘ 𝟙)%T v1 v2 }}.*)
                               (∀ᵣ θ₁, ∀ᵣ θ₂,  (((𝔾 × (𝟙 + 𝟙)) -{ θ₁ }-> 𝟙) × ((𝟙 + 𝟙) -{ θ₁ }-> Option 𝟙)) ⊸ (((𝟙 + 𝟙) -{ θ₂ }-> 𝟙) ×(𝟙 + 𝟙) -{ θ₂ }-> Option 𝟙) -{ sem_row_union θ₁ (sem_row_union θ₂ L) }-∘ 𝟙)%T v1 v2 }}.
-Proof with (repeat foldkont) using G.
- Admitted.
+Proof with (repeat foldkont) using  Bdd_int_vg Bij_log Bij_xor_sem Bij_xor_sem_l G H
+Val_log XOR_spec0 cg group_xor_sem log__g vg
+vg_int_xor_sem vgg xor_struct Σ.
+
+ iIntros "Hrelf1f2".  
+  repeat simpl. 
+  unfold R_CHAN. brel_pures.
+  unfold right_composition. brel_pures.
+  unfold CHAN.
+  repeat simpl. brel_pures'.
+  
+
+  unfold F_CHAN, CHAN_SIM_lazy. 
+   
+  repeat simpl. brel_pures. iModIntro. iIntros (autheff keyeff). 
+  simpl.
+  iIntros (autheff_l autheff_r) "Hautheff".
+  iDestruct "Hautheff" as (asnd_l asnd_r arcv_l arcv_r) "(%H1al & %H2al & (#Hasnd & #Harcv))".
+  brel_pures. iModIntro.
+  iIntros (keyeff_l keyeff_r) "Hkeyeff".
+  iDestruct "Hkeyeff" as (kysnd_l kysnd_r kyrcv_l kyrcv_r) "(%H1k & %H2k & (#Hkeysnd & #Hkeyrcv))".
+  rewrite H1al. rewrite H2al. rewrite H1k. rewrite H2k.
+  brel_pures.
+  unfold F_OAUTH, F_KE_lazy_alice.
+  brel_pures.  
+
+  iApply brel_alloc_l. iIntros (l_sim) "!> Hl_sim". brel_pures_l.
+  iApply brel_alloc_l. iIntros (l_m'sim) "!> Hl_m'sim". brel_pures_l.
+  iApply brel_alloctape_r. iIntros (γ) "Hγ". brel_pures_r.
+  iApply brel_alloc_r. iIntros (l_key) "Hl_key". brel_pures_r.
+   iApply brel_effect_r. iIntros (getKey') "HgK !>". brel_pures_r.
+  iApply brel_effect_l. iIntros (leaksec') "!> Hleaksec !>". brel_pures.
+  iApply brel_alloc_r. iIntros (l_auth) "Hl_auth". brel_pures_r.
+  iApply brel_effect_r. iIntros (channel') "Hchannel !>". brel_pures_r.
+  
+ 
+  iApply brel_alloc_l. iIntros (l_fchan) "!> Hlfchan". brel_pures_l.
+  iApply brel_effect_l. iIntros (schannel_l) "!> Hschannel_l !>". brel_pures_l.
+  brel_pures'. repeat simpl. brel_pures'.
+  iApply brel_alloc_r. iIntros (l_rchan) "Hlrchan". brel_pures_r.
+  iApply brel_effect_r. iIntros (schannel_r) "Hschannel_r !>". brel_pures_r.  
+  set (kl1 := ( match: "payload" with
+         InjL "m" =>
+           match: ! #l_rchan with
+             InjL <> =>
+               #l_rchan <- InjR "m";; 
+               let: "key" := (λ: "party", do: getKey' "party")%V bob in
+               match: "key" with
+                 InjL <> => "k" #()%V
+               | InjR "x" =>
+                 match: G_XOR xor "m" "x" with
+                   InjL <> => "k" #()%V
+                 | InjR "mg" =>
+                   (λ: "m", do: channel' InjL "m")%V ("mg", bob);; "k" #()%V
+                 end
+               end
+           | InjR "m" => "k" #()%V
+           end
+       | InjR <> =>
+         let: "key" := (λ: "party", do: getKey' "party")%V alice in
+         match: "key" with
+           InjL <> => "k" (InjLV #()%V)
+         | InjR "key" =>
+           let: "r" := (λ: "m", do: channel' InjR "m")%V bob in
+           match: "r" with
+             InjL <> => "k" (InjLV #()%V)
+           | InjR "x" =>
+             match: G_XOR xor "x" "key" with
+               InjL <> => "k" (InjL #()%V)
+             | InjR "mg" => "k" (InjR "mg")
+             end
+           end
+         end
+       end )%E ).
+  set (kl2 := ( match: "payload" with
+         InjL "payload" =>
+           let: "dst" := "payload" in
+           let: "m" := Fst "dst" in
+           let: "dst" := Snd "dst" in
+           match: ! #l_auth with
+             InjL <> => #l_auth <- InjR "m";; asnd_l ("m", "dst");; "k" #()%V
+           | InjR "message" => "k" #()%V
+           end
+       | InjR "from" =>
+         let: "r" := arcv_l "from" in
+         match: "r" with
+           InjL <> => "k" (InjLV #()%V)
+         | InjR "x" => "k" ! #l_auth
+         end
+       end )%E).
+  set (kl3 := ( match: "p" with
+         InjL <> =>
+           let: "key" := (λ: <>,
+                            match: ! #l_key with
+                              InjL <> =>
+                                let: "c" := #();; rand(#lbl:γ) #(S n'') in
+                                let: "key" := vexp g "c" in
+                                #l_key <- InjR "key";; "key"
+                            | InjR "key" => "key"
+                            end)%V
+                           #()%V in
+           kysnd_l bob;; 
+           let: "r" := kyrcv_l bob in
+           match: "r" with
+             InjL <> => "k" (InjLV #()%V)
+           | InjR "w" => "k" (InjR "key")
+           end
+       | InjR <> =>
+         let: "r" := kyrcv_l alice in
+         match: "r" with
+           InjL <> => "k" (InjLV #()%V)
+         | InjR "w" =>
+           kysnd_l alice;; 
+           match: ! #l_key with
+             InjL <> => "k" (InjLV #()%V)
+           | InjR "key" => "k" (InjR "key")
+           end
+         end
+       end )%E).
+  set (kr1 := ( match: "payload" with
+         InjL "m" =>
+           match: ! #l_fchan with
+             InjL <> =>
+               #l_fchan <- InjR "m";; 
+               (λ: "m", do: leaksec' InjL "m")%V alice;; "k" #()%V
+           | InjR "x" => "k" #()%V
+           end
+       | InjR <> =>
+         let: "r" := (λ: "m", do: leaksec' InjR "m")%V bob in
+         match: "r" with
+           InjL <> => "k" (InjLV #()%V)
+         | InjR "x" => "k" (InjR ! #l_fchan)
+         end
+       end )%E).
+  set (kr2 := ( match: "payload" with
+         InjL <> =>
+           let: "m'" := (λ: <>,
+                           match: ! #l_m'sim with
+                             InjL <> =>
+                               let: "m'" := #();; rand #(S n'') in
+                               #l_m'sim <- InjR "m'";; "m'"
+                           | InjR "m'" => "m'"
+                           end)%V
+                          #()%V in
+           kysnd_r bob;; 
+           let: "r" := kyrcv_r bob in
+           match: "r" with
+             InjL <> => "k" (InjLV #()%V)
+           | InjR "x" =>
+             match: ! #l_sim with
+               InjL <> =>
+                 let: "mA" := vexp g "m'" in
+                 #l_sim <- InjR "m'";; asnd_r ("mA", bob);; "k" #()%V
+             | InjR "m" => "k" #()%V
+             end
+           end
+       | InjR <> =>
+         let: "r" := kyrcv_r alice in
+         match: "r" with
+           InjL <> => "k" (InjLV #()%V)
+         | InjR "x" =>
+           kysnd_r alice;; 
+           match: ! #l_m'sim with
+             InjL <> => "k" (InjLV #()%V)
+           | InjR "_" =>
+             let: "rla" := arcv_r bob in
+             match: "rla" with
+               InjL <> => "k" (InjLV #()%V)
+             | InjR "x" => "k" ! #l_sim
+             end
+           end
+         end
+                end )%E).
+  set (θ := client_row' channel' leaksec' getKey' schannel_l schannel_r).
+  iSpecialize ("Hrelf1f2" $! θ).
+  unfold sem_ty_arr, sem_ty_mbang. simpl.
+  iAssert (sem_val_typed  ((λ: "m", do: schannel_l InjL "m"), (λ: <>, do: schannel_l InjR bob))%V ((λ: "m", do: schannel_r InjL "m") , (λ: <>, do: schannel_r InjR bob))%V (((𝔾 -{ θ }-> 𝟙) × (𝟙 -{ θ }-> (Option 𝔾)))%T)) as "Hschn".
+  {
+      unfold sem_val_typed. simpl. intros. 
+    iModIntro. rewrite /sem_ty_arr /sem_ty_mbang /sem_ty_option /sem_ty_sum //=. rewrite /sem_ty_prod. 
+    iExists (λ: "m", do: schannel_l InjL "m")%V , (λ: "m", do: schannel_r InjL "m")%V , (λ: <>, do: schannel_l InjR bob)%V , (λ: <>, do: schannel_r InjR bob)%V.  repeat iSplit; try iPureIntro; try auto.
+    + iModIntro. iIntros (??) "Hw1w1". brel_pures.
+      iApply brel_introduction'; try constructor;
+      iExists _,_,[],[],_; do 2 (iSplit; [by iPureIntro|]; iSplit; [iPureIntro; apply NeutralEctx_nil|]);
+      iSplit; try (iIntros (??) "!# H"; iApply "H").
+      simpl. iLeft. unfold sem_ty_group.  
+      iDestruct "Hw1w1" as (g) "[%Hw1 %Hw2]".  
+      iExists _. repeat iSplit; try iPureIntro; try auto; unfold SendV; try rewrite -> Hw1;
+      try rewrite -> Hw2; try reflexivity.
+      iModIntro. iApply brel_value. iIntros "$ !>".
+      unfold sem_ty_unit; iPureIntro.
+      split; reflexivity.
+    + iModIntro. iIntros (??) "Hw1w1". unfold sem_ty_unit. 
+      iDestruct "Hw1w1" as "[%Hw1 %Hw2]". unfold bob. rewrite -> Hw1. rewrite -> Hw2.
+      brel_pures.
+      iApply brel_introduction'; try constructor. 
+      iExists _,_,[],[],_; do 2 (iSplit; [by iPureIntro|]; iSplit; [iPureIntro; apply NeutralEctx_nil|]);
+      iSplit; try (iIntros (??) "!# H"; iApply "H").     simpl. iRight.
+      repeat iSplit; try iPureIntro; try auto; unfold RecvV; unfold bob; try rewrite -> Hw1;
+        try rewrite -> Hw2; try simpl; try reflexivity.
+      iModIntro. iSplit.  
+      { iIntros (?). iApply brel_value. iIntros "$ !>".
+        iExists _,_; iRight; iPureIntro; repeat (split; first done). exists g. split; reflexivity. }
+      { iApply brel_value. iIntros "$ !>".
+        iExists _,_; iLeft; iPureIntro; repeat (split; first done); reflexivity. }
+  }
+  unfold sem_val_typed. simpl.
+  iDestruct "Hschn" as "#Hschn".
+  iSpecialize ("Hrelf1f2" with "Hschn"). simpl.
+  set (f m := (fun (x : nat) =>
+                 match (decide (x < S (S n'')))%nat with
+                 | left H =>  fin_to_nat (log__g (group_xor_sem m (g ^+(nat_to_fin H))))
+                 | right _ => x
+                 end )).
+  assert (Hf : ∀ m : vgG, @Bij nat nat (f m)).
+  {
+    intro m.
+     set (f' m := (λ n : fin (S (S n'')),
+         log__g (group_xor_sem m (g ^+ n)))).
+pose proof (Bij_log m) as [Hinj_fin Hsurj_fin].
+split.
+- intros x y Hxy. unfold f in Hxy.
+  case_decide as Hx; case_decide as Hy.
+  + 
+    apply fin_to_nat_inj in Hxy.
+    apply (inj _ (Inj := Hinj_fin)) in Hxy.   
+    apply (f_equal fin_to_nat) in Hxy.
+    rewrite !fin_to_nat_to_fin in Hxy. exact Hxy.
+  + 
+    exfalso.
+   
+    pose proof (fin_to_nat_lt (f' m (nat_to_fin Hx))).
+    unfold f' in H0. rewrite -> Hxy in H0.  lia. 
+  + 
+    exfalso.
+    pose proof (fin_to_nat_lt (f' m (nat_to_fin Hy))).
+    unfold f' in H0. rewrite <- Hxy in H0. lia.
+  + exact Hxy.
+- intros z. unfold f.
+  destruct (decide (z < S (S n''))%nat) as [Hz | Hz].
+  + destruct (Hsurj_fin (nat_to_fin Hz)) as [i Hi].
+    exists (fin_to_nat i).
+    case_decide as Hi'; [| pose proof (fin_to_nat_lt i); lia].
+    rewrite fin_to_nat_to_fin.
+    rewrite Hi.
+    by rewrite fin_to_nat_to_fin.
+  + exists z. case_decide; [lia | reflexivity].
+  }
+  set (d1 := (γ ↪ₛN (S n''; []) ∗ l_m'sim ↦ NONEV ∗ l_sim ↦ NONEV ∗ l_auth ↦ₛ NONEV ∗ l_fchan ↦ NONEV ∗ l_rchan ↦ₛ NONEV ∗  l_key ↦ₛ NONEV)%I).
+  set (d2 := ((∃ m : vgG, ∃ n : nat, γ ↪ₛN (S n''; []) ∗ l_m'sim ↦□ SOMEV #n ∗ l_sim ↦□ SOMEV #n ∗
+                  l_auth ↦ₛ□ SOMEV (vgval
+                                     (group_xor_sem m (g ^+(f m n))))%V ∗  l_fchan ↦□ SOMEV (vgval m) ∗  l_rchan ↦ₛ□ SOMEV (vgval m) ∗ l_key ↦ₛ□ SOMEV (vgval (g ^+(f m n))))%I)).
+
+  set (d3 := (∃ m : vgG, ∃ n : nat, γ ↪ₛN (S n''; []) ∗ l_m'sim ↦□ SOMEV #n ∗ l_sim ↦ NONEV ∗ l_auth ↦ₛ NONEV ∗ l_fchan ↦□ SOMEV (vgval m) ∗  l_rchan ↦ₛ□ SOMEV (vgval m) ∗ l_key ↦ₛ□ SOMEV (vgval (g ^+(f m n))))%I). 
+  iApply (brel_na_alloc (d1 ∨ (d2 ∨ d3))%I alphaN).
+  iSplitL "Hγ Hl_m'sim Hl_sim Hl_auth Hlfchan Hlrchan Hl_key"; [iNext; iLeft; iFrame|].
+  { iPureIntro. auto. }
+   iIntros "#Hinvα".
+   iApply brel_new_theory.
+   iApply (brel_add_label_l with "Hschannel_l").
+   iApply (brel_add_label_r with "Hschannel_r").
+   iApply (brel_add_label_r with "HgK").
+   iApply (brel_add_label_r with "Hchannel").
+   iApply (brel_add_label_l with "Hleaksec").
+   set (X :=  iLblSig_to_iLblThy [([schannel_l] , [schannel_r] , sec_channel schannel_l schannel_r)]).
+   set (R := (λ u1 u2 : val, 𝟙%T u1 u2)).
+   set (X' := sec_channel schannel_l schannel_r).
+   iApply brel_learn. iIntros "%Hdist' _".
+   iApply ((brel_exhaustion (f1 ((λ: "m", do: schannel_l InjL "m"),(λ: <>, do: schannel_l InjR bob))%V) (f2 ((λ: "m", do: schannel_r InjL "m"),(λ: <>, do: schannel_r InjR bob))%V) _ _ X' _ _ R _ _ _) with "[Hrelf1f2]").
+   {  simpl. set_solver. }
+   { simpl. set_solver. }   
+   {
+     set clt := ([leaksec'; schannel_l], [channel'; getKey'; schannel_r], X').
+     set cltheory := iLblSig_to_iLblThy [([leaksec'; schannel_l] , [channel'; getKey'; schannel_r] , X')].
+     set (L' := cltheory ++ (iLblSig_to_iLblThy L)).
+    (* set (keytheory := iLblSig_to_iLblThy [([keyleak1], [keyleak2], keyleak keyleak1 keyleak2)]).
+     set (leaktheory := (iLblSig_to_iLblThy [([leakauth1], [leakauth2], leakauth leakauth1 leakauth2)])).*)
+     set (keytheory := keyeff).
+     set (leaktheory := autheff).
+     set (M := cltheory ++ (iLblSig_to_iLblThy (sem_row_union leaktheory (sem_row_union keytheory L)))).
+      iApply (brel_introduction_mono L' M).
+     + simpl.
+       iApply to_iThy_le_intro'.
+       unfold L'. unfold M.
+       set (ρ__c := (sem_row_union leaktheory (sem_row_union keytheory L))).
+       apply (submseteq_skips_l cltheory (iLblSig_to_iLblThy L) (iLblSig_to_iLblThy ρ__c)).
+       unfold ρ__c. unfold sem_row_union. repeat (rewrite -> iLblSig_to_iLblThy_proj; rewrite -> iLblSig_to_iLblThy_app).
+       solve_submseteq.
+     + unfold L'. unfold cltheory. simpl. iApply "Hrelf1f2". } 
+    iLöb as "IH".
+   unfold kl1.
+   iSplit; [iIntros (v1 v2) "%Hv1v2"; iModIntro; brel_pures; iModIntro; done |].  
+   iIntros (?????) "!# %Hk1 %Hk2 HXQ #Hrel".  
+   iDestruct "HXQ" as "[HSendAlice | HRecvBob]". 
+   (* Send a message using the secure channel from Alice To Bob *)
+   + iDestruct "HSendAlice" as (?m) "[[%He1 %He2] #HmQ]".
+      rewrite -> He1. rewrite -> He2. brel_pures.
+      { apply -> NeutralEctx_ectx_labels_singleton.
+         eapply NeutralEctx_label_cons_inv_2 in Hk1.
+         eapply NeutralEctx_label_cons_inv_1 in Hk1. eapply Hk1. }
+    {  apply -> NeutralEctx_ectx_labels_singleton.
+       do 2 (eapply NeutralEctx_label_cons_inv_2 in Hk2). eapply Hk2. } 
+         iApply (brel_na_inv _ _ alphaN); first set_solver.
+         iFrame "Hinvα".
+           iIntros "([(>Hγ & >Hl_m'sim & >Hl_sim & >Hl_auth & >Hl_fchan & >Hl_rchan & >Hl_key) | [>Hd2 | >Hd3 ]] & Hclose)".
+          (* First message to be sent by the secure channel*)
+        ++ 
+           iApply (brel_load_l _ _ _ [HandleCtx _ _ _ _ _ ; CaseCtx _ _] with "Hl_fchan").
+           iIntros "!>Hl_fchan".
+           iApply (brel_load_r _ _ _ _ [HandleCtx Deep MS getKey' _ _ ; HandleCtx Deep MS channel' _ _; CaseCtx _ _] with "Hl_rchan").
+           iIntros "Hl_rchan". brel_pures.
+           simpl. brel_pures. 
+           iApply (brel_store_l _ _ _ [HandleCtx _ _ _ _ _ ; AppRCtx _] with "Hl_fchan"). iIntros "!>Hl_fchan".
+           simpl.
+           brel_pures.
+           { simpl. apply not_elem_of_nil. }
+           iApply (brel_store_r _ _ _ _ [HandleCtx _ _ _ _ _ ; HandleCtx _ _ _ _ _ ; AppRCtx _] with "Hl_rchan"). 
+           iIntros "Hl_rchan". brel_pures; try (simpl); try (apply not_elem_of_nil).
+           { unfold distinct in Hdist'. destruct Hdist'. unfold distinct_r in H1.
+                        simpl in H1.
+                        repeat (rewrite -> labels_l_cons in H1).
+                        eapply NoDup_app in H1.
+                        eapply NoDup_cons_1_1. destruct H1.
+                        eapply (submseteq_NoDup _ [channel'; getKey'; schannel_r]); [solve_submseteq | apply H1]. }
+           repeat foldkont.
+           iApply (brel_load_r _ _ _ _ [AppRCtx _ ; CaseCtx _ _] with "Hl_key"). iIntros "Hl_key".
+           brel_pures_r.
+           iApply (brel_load_l _ _ _ [AppRCtx _ ; CaseCtx _ _] with "Hl_m'sim"). iIntros "!> Hl_m'sim".
+           brel_pures.
+           iDestruct "Hγ" as (ms) "(%Hf' & Hγ)". apply map_eq_nil in Hf'. simplify_eq.
+           iApply (brel_couple_UT _ _ (f m) [AppRCtx _; AppRCtx _] _ _ _ _ _ _).
+           1: auto.
+           { intros. unfold f. case_decide as Hn.
+             + apply fin_to_nat_lt.
+             + contradiction. }
+           iFrame "Hγ". simpl. iSplit => //. iIntros (c ?) "!> Hγ".
+          (*simpl. iSplitL "Hγ". {iModIntro ; iFrame "Hγ". iPureIntro. auto. } 
+          iIntros (c) "!> Hc Hγ". *)
+          brel_pures.
+          iApply (brel_store_l _ _ _ [AppRCtx _; AppRCtx _] with "Hl_m'sim").
+           iIntros "!> Hl_m'sim". brel_pures. simpl. 
+           About brel_randT_r.
+           About brel_randT_l.
+           iApply (brel_randT_r _ [AppRCtx _ ; AppRCtx _] with "Hγ").
+           iIntros "Hγ %Hc".
+           brel_pures.
+           simpl.
+           iApply (brel_exp_r [AppRCtx _ ; AppRCtx _] _ _ _ g (f m c) _).
+           brel_pures.
+           iApply (brel_store_r _ _ _ _ [AppRCtx _; AppRCtx _ ] with "Hl_key"). iIntros "Hl_key".
+          
+           iApply fupd_brel.
+           iMod (ghost_map_elem_persist with "Hl_fchan") as "#Hl_fchan".
+           iMod (ghost_map_elem_persist with "Hl_rchan") as "#Hl_rchan".
+           iMod (ghost_map_elem_persist with "Hl_key") as "#Hl_key".
+           iMod (ghost_map_elem_persist with "Hl_m'sim") as "#Hl_m'sim".
+           iModIntro.
+           iApply brel_na_close. iFrame.
+           iSplitL.
+           { iModIntro. iRight. iRight. unfold d3.  iExists m, c.
+             iFrame "Hγ Hl_m'sim Hl_sim Hl_auth Hl_fchan Hl_rchan Hl_key". }
+           (* set (keytheory := iLblSig_to_iLblThy [([keyleak1], [keyleak2], keyleak keyleak1 keyleak2)]).*)
+            set (keytheory := keyeff).
+            (* set (leaktheory := (iLblSig_to_iLblThy [([leakauth1], [leakauth2], leakauth leakauth1 leakauth2)])).*)
+            set (leaktheory := autheff).
+            set (M := [([leaksec'; schannel_l], [channel'; getKey';  schannel_r], @iThyBot Σ)] ++ (iLblSig_to_iLblThy (sem_row_union leaktheory L))).
+            set (N := [([leaksec'; schannel_l], [channel'; getKey'; schannel_r], @iThyBot Σ)] ++ (iLblSig_to_iLblThy (sem_row_union leaktheory (sem_row_union keytheory L)))).
+            brel_pures.
+             iApply (brel_bind'' [ AppRCtx _] [AppRCtx _] (iLblSig_to_iLblThy keytheory) M N (𝟙%T) (kysnd_l bob) (kysnd_r bob)).
+             { simpl. set_solver. }
+             { simpl. set_solver. }
+             { simpl. unfold M. unfold N. iApply to_iThy_le_intro'. 
+               unfold sem_row_union. repeat (rewrite -> iLblSig_to_iLblThy_proj; rewrite -> iLblSig_to_iLblThy_app).
+               solve_submseteq. }
+             {
+               iApply (brel_wand _ _ _  R _ ).
+               { iDestruct "Hkeysnd" as "#Hkeysnd".
+                 iSpecialize ("Hkeysnd" $! bob bob).
+                 iApply "Hkeysnd".
+                 { unfold sem_ty_sum, sem_ty_unit. unfold bob. iExists #()%V, #()%V.
+                   iLeft. repeat (iSplit); try (iPureIntro); try reflexivity. } }
+               iModIntro. iIntros (v1 v2) "#HRv1v2".
+               brel_pures.
+                iApply (brel_bind'' _ _ (iLblSig_to_iLblThy keytheory) M N 𝟙%T (kyrcv_l bob) (kyrcv_r bob)).
+                { simpl. unfold M.  repeat (rewrite -> labels_l_cons). set_solver. }
+                { simpl. apply list_subseteq_nil. }
+                { simpl. unfold M. unfold N. iApply to_iThy_le_intro'.
+                  unfold sem_row_union. repeat (rewrite -> iLblSig_to_iLblThy_proj; rewrite -> iLblSig_to_iLblThy_app).
+               solve_submseteq. }
+                (*iApply (brel_introduction' [keyleak1] [keyleak2]).*)
+                iApply brel_wand.
+                { iDestruct "Hkeyrcv" as "#Hkeyrcv".
+                  iSpecialize ("Hkeyrcv" $! bob bob).
+                  iApply "Hkeyrcv".
+                  { unfold bob. unfold sem_ty_sum. iExists #()%V, #()%V.
+                    repeat iSplit; try (iPureIntro); try reflexivity; try (left); repeat split;
+                      try reflexivity. } }
+                iModIntro. iIntros (v0 v3) "#Hv0v3".
+                unfold sem_ty_group, sem_ty_option, sem_ty_sum.
+                iDestruct "Hv0v3" as (?w1 ?w2) "#Hv0v3".
+                (* keyleak recv returns succesfully or not *)
+                iDestruct "Hv0v3" as "[Hnone | Hsome]".
+               ++ iDestruct "Hnone" as "(%Hv0 & (%Hv3 & Hw1w2))".
+                  rewrite -> Hv0. rewrite -> Hv3. unfold sem_ty_unit.
+                  iDestruct "Hw1w2" as "(%Hw1 & %Hw2)".
+                  rewrite -> Hw1. rewrite -> Hw2.
+                  brel_pures.
+                   iApply (brel_exhaustion (fill k1' #()%V) (fill k2' #()%V)). 
+                      { simpl. auto. }
+                      { simpl. repeat (eapply list_subseteq_skip). set_solver. }
+                      { iApply "Hrel". iApply "HmQ". }
+                      { iApply "IH". }
+               ++ iDestruct "Hsome" as "(%Hv0 & (%Hv3 &Hw1w2))".
+                  rewrite -> Hv0. rewrite -> Hv3.
+                  unfold sem_ty_unit.
+                  iDestruct "Hw1w2" as "(%Hw1 & %Hw2)".
+                  rewrite -> Hw1. rewrite -> Hw2.
+                  brel_pures.
+                  iApply G_XOR_CORRECT_r.
+                  { rewrite -> vg_int_xor_sem.  repeat (rewrite -> Bij_xor_sem). reflexivity. }
+                  brel_pures.
+                  { simpl. set_solver.  }
+                        iApply (brel_na_inv _ _ alphaN); first set_solver.
+                        iFrame "Hinvα".
+                        iIntros "([ (>Hγ & (>Hl_m'sim' & (>Hl_sim' & (>Hl_auth & (>Hl_fchan' & (>Hl_rchan' & Hl_key')))))) | [>Hd2 | >Hd3]] & Hclose)".
+                         (*contradiction branch as the first message has been sent and stored*)
+                          - iDestruct (ghost_map_elem_agree
+                                        with "Hl_fchan Hl_fchan'") as %Heq.
+                            congruence.
+                          -
+                            unfold d2. 
+                            iDestruct "Hd2" as (?m ?n) "(Hγ & (Hl_m'sim' & (Hl_sim & (Hl_auth & (Hl_fchan' & (Hl_rchan' & Hl_key'))))))". 
+                            iApply (brel_load_r _ _ _ _ [HandleCtx _ _ _ _ _ ;CaseCtx _ _] with "Hl_auth").                                          
+                          iIntros "Hl_auth".
+                          simpl. brel_pures_r.
+                          iApply (brel_load_l _ _ _ [CaseCtx _ _] with "Hl_sim").
+                          iIntros "!> Hl_sim". brel_pures. simpl.
+                          iApply fupd_brel.
+                          iModIntro.
+                          iApply brel_na_close. iFrame "Hclose".
+                          iSplitL.
+                          { iModIntro. iRight. iLeft. iFrame "Hγ Hl_m'sim' Hl_sim Hl_auth Hl_fchan' Hl_rchan' Hl_key'". }
+                         
+                            brel_pures. 
+                            iApply (brel_exhaustion (fill k1' #()%V) (fill k2' #()%V)).
+                            { simpl. auto. }
+                            { simpl. auto. set_solver. }
+                            { iApply "Hrel". iApply "HmQ". }
+                            { iApply "IH". }
+                        - unfold d3.
+                          iDestruct "Hd3" as (?m ?n) "(Hγ & (Hl_m'sim' & (Hl_sim & (Hl_auth & (Hl_fchan' & (Hl_rchan' & Hl_key'))))))". 
+                          iApply (brel_load_r _ _ _ _ [HandleCtx _ _ _ _ _ ;CaseCtx _ _] with "Hl_auth").                                          
+                          iIntros "Hl_auth".
+                          simpl. brel_pures_r.
+                          iApply (brel_load_l _ _ _ [CaseCtx _ _] with "Hl_sim").
+                          iIntros "!> Hl_sim". brel_pures. simpl.
+                          iApply (brel_exp_l [AppRCtx _]). brel_pures.                     
+                          iApply (brel_store_l _ _ _ [AppRCtx _] with "Hl_sim").
+                          iIntros "!> Hl_sim". rel_pures. 
+                          iApply (brel_store_r _ _ _ _ [HandleCtx _ _ _ _ _ ; AppRCtx _] with "Hl_auth").
+                          iIntros "Hl_auth". brel_pures.
+                          iApply fupd_brel.
+                          iMod (ghost_map_elem_persist with "Hl_sim") as "#Hl_sim".
+                          iMod (ghost_map_elem_persist with "Hl_auth") as "#Hl_auth".
+                          iDestruct "Hγ" as (ns) "(%Hfγ & Hγ)".
+                          apply map_eq_nil in Hfγ. simplify_eq. 
+                         (* iMod (ghost_map_elem_persist with "Hγ") as "#Hγ".*)
+                          iModIntro.
+                          iApply brel_na_close. iFrame.
+                          iSplitL.
+                          { iModIntro. iRight. iLeft. iExists m, c. iFrame "#". iPureIntro; auto. }
+                          simpl. brel_pures.
+                          set (g_sem := (group_xor_sem m (valgroup.g ^+ f m c))).
+                          repeat foldkont.
+                          unfold kl3.
+                          set (hbranchright := (λ: "p" "k",
+                           match: "p" with
+                           InjL <> =>
+                           let: "key" := (λ: <>,
+                            match: ! #l_key with
+                              InjL <> =>
+                                let: "c" := 
+                                #();; 
+                                rand(#lbl:γ) #
+                                (S n'') in
+                                let: "key" := 
+                                vexp g "c" in
+                                #l_key <-
+                                InjR "key";; "key"
+                            | InjR "key" => "key"
+                            end)%V
+                           #()%V in
+                           kysnd_r bob;; 
+                           let: "r" := kyrcv_r bob in
+                           match: "r" with
+                             InjL <> => "k" (InjLV #()%V)
+                           | InjR "w" => "k" (InjR "key")
+                           end
+                            | InjR <> =>
+                               let: "r" := kyrcv_r alice in
+                                match: "r" with
+                                InjL <> => "k" (InjLV #()%V)
+                              | InjR "w" =>
+                                kysnd_r alice;; 
+                                match: ! #l_key with
+                                InjL <> => "k" (InjLV #()%V)
+                               | InjR "key" => "k" (InjR "key")
+                                 end
+                                 end end )%E).
+             
+                          iPoseProof (brel_bind [AppRCtx (λ: <>, kont #()%V)]
+                                     [HandleCtx Deep MS getKey' hbranchright (λ: "y", "y"); AppRCtx (λ: <>, kont1 #()%V)] ⊤ (iLblSig_to_iLblThy leaktheory) N  𝟙%T
+                      (asnd_l (vgval (g ^+c), bob))%V
+                      (asnd_r (vgval g_sem, bob))%V) as "Hbind".
+                        iApply "Hbind".
+                         (* iApply (brel_bind [HandleCtx _ _ _ _ _ ; AppRCtx _] [AppRCtx _] ⊤ (iLblSig_to_iLblThy leaktheory)
+                                    N _ (asnd_l (InjLV (vgval g_sem, bob)))
+                            (asnd_r (InjLV (vgval (valgroup.g ^+ f m c), bob)))).*)
+                         { simpl. unfold leaktheory. auto.
+                            iApply (traversable_ectx_labels _ _ [] [getKey'] iThyBot _). 
+                            + simpl. auto.
+                            + unfold kont1. simpl. auto.
+                            + simpl.
+                              unfold sem_row_union in Hdist'.
+                              unfold distinct in *.
+                              unfold distinct_l, distinct_r in *.
+                              unfold labels_l, labels_r in *.
+                              destruct Hdist' as [Hl Hr].
+                              split.
+                              ++ 
+                                set (l1 := (concat  (([], [getKey'], iThyBot) :: iLblSig_to_iLblThy autheff).*1.*1)).
+                                 eapply (submseteq_NoDup l1 _); try eapply Hl.
+                                 unfold l1. simpl. eapply submseteq_cons. (*eapply submseteq_skip.*)
+                                  repeat (rewrite -> iLblSig_to_iLblThy_proj;
+                                          rewrite -> iLblSig_to_iLblThy_app). 
+                                  repeat (rewrite -> fmap_app). simpl. eapply submseteq_cons. 
+                                  eapply concat_submseteq. simpl. solve_submseteq.
+                              ++ set (l2 := (concat (([], [getKey'], iThyBot)
+                                  :: iLblSig_to_iLblThy autheff).*1.*2)).
+                                 eapply (submseteq_NoDup l2 _); try eapply Hr.
+                                 unfold l2. simpl. (*eapply submseteq_skip.*)
+                                 eapply submseteq_cons. eapply submseteq_skip.
+                                  repeat (rewrite -> iLblSig_to_iLblThy_proj;
+                                          rewrite -> iLblSig_to_iLblThy_app). 
+                                  repeat (rewrite -> fmap_app). simpl.  eapply submseteq_cons.
+                                  eapply concat_submseteq. simpl. solve_submseteq.
+                            }
+                            { simpl. unfold N. iApply to_iThy_le_intro'. 
+                              unfold sem_row_union. repeat (rewrite -> iLblSig_to_iLblThy_proj; rewrite -> iLblSig_to_iLblThy_app).
+                              solve_submseteq. }
+                            {  iApply (brel_wand _ _ _ R _).
+                            {  iDestruct "Hasnd" as "#Hasnd".
+                               iSpecialize ("Hasnd" $! (vgval (g ^+c), bob)%V).
+                               iSpecialize ("Hasnd" $! (vgval g_sem, bob)%V).
+                               iApply "Hasnd".
+                               unfold g_sem. simpl. unfold sem_ty_prod.
+                               iExists (vgval (valgroup.g ^+ c)) , (vgval (group_xor_sem m (valgroup.g ^+ f m c))) , bob , bob.
+                               repeat (iSplit); try (iPureIntro); try reflexivity.
+                               + auto. simpl. unfold f. case_decide as Hc'; [| exfalso; lia].
+                                 rewrite -> Val_log.
+                                 rewrite -> Bij_xor_sem_l.
+                                 assert (fin_to_nat (nat_to_fin Hc') = c)
+                                 as -> by apply fin_to_nat_to_fin.
+                                 exists (g ^+ c)%g.
+                                 repeat split; reflexivity.
+                               + simpl. exists #()%V, #()%V. repeat split; unfold bob; try reflexivity.
+                                 left. repeat split; reflexivity. }
+                            iModIntro. iIntros (v0 v3) "#HRv0v3".
+                            unfold R. unfold sem_ty_unit.
+                            iDestruct "HRv0v3" as "(%Hv0 & %Hv3)".
+                            rewrite -> Hv0. rewrite -> Hv3.
+                            brel_pures.
+                            iApply (brel_exhaustion (fill k1' #()%V) (fill k2' #()%V)).
+                            { simpl. auto. }
+                            { simpl. set_solver. }
+                            { iApply "Hrel". iApply "HmQ". }
+                            { iApply "IH". } } }
+        (* A message has already been sent by the secure channel *)     
+        ++ unfold d2.
+           iDestruct "Hd2" as (?m ?n) "(Hγ & (Hl_m'sim & (Hl_sim & (Hl_auth & (Hl_fchan & (Hl_rchan & Hl_key))))))".
+           iDestruct "Hl_fchan" as "#Hl_fchan".
+           iDestruct "Hl_rchan" as "#Hl_rchan".
+           iApply (brel_load_r _ _ _ _  [HandleCtx _ _ _ _ _ ; HandleCtx _ _ _ _ _ ; CaseCtx _ _] with "Hl_rchan").
+           iIntros "Hl_rchan'".
+           brel_pures.
+           iApply (brel_load_l _ _ _ [HandleCtx _ _ _ _ _ ; CaseCtx _ _] with "Hl_fchan").
+           iIntros "!> Hl_fchan'".
+           brel_pures.
+           iApply brel_na_close. iFrame.
+           iSplitL.
+           { iModIntro. iRight. iLeft. iFrame. }
+           iApply (brel_exhaustion (fill k1' #()%V) (fill k2' #()%V)).
+           { simpl. auto. }
+           { simpl. set_solver. }
+           { iApply "Hrel". iApply "HmQ". }
+           { iApply "IH". }         
+        ++ unfold d3.
+           iDestruct "Hd3" as (?m ?n) "(Hγ & (Hl_m'sim & (Hl_sim & (Hl_auth & (Hl_fchan & (Hl_rchan & Hl_key))))))".
+           iApply (brel_load_r _ _ _ _ [HandleCtx _ _ _ _ _ ; HandleCtx _ _ _ _ _ ; CaseCtx _ _] with "Hl_rchan").
+           iIntros "Hl_rchan'".
+           brel_pures.
+           iApply (brel_load_l _ _ _  [HandleCtx _ _ _ _ _ ; CaseCtx _ _] with "Hl_fchan").
+           iIntros "!> Hl_fchan'".
+           brel_pures.
+           iApply brel_na_close. iFrame.
+           iSplitL.
+           { iModIntro. iRight. iRight. iFrame. }
+           iApply (brel_exhaustion (fill k1' #()%V) (fill k2' #()%V)).
+           { simpl. auto. }
+           { simpl. set_solver. }
+           { iApply "Hrel". iApply "HmQ". }
+           { iApply "IH". }
+           
+        + iDestruct "HRecvBob" as "[%He1 [%He2 #HmQ]]".  
+     rewrite -> He1. rewrite -> He2. brel_pures.
+     { split.
+       + apply -> NeutralEctx_ectx_labels_singleton.
+         (eapply NeutralEctx_label_cons_inv_2 in Hk1). eapply Hk1.
+       + simpl.  set_solver.  }
+     { split.
+       + apply -> NeutralEctx_ectx_labels_singleton.
+           do 2 (eapply NeutralEctx_label_cons_inv_2 in Hk2).
+           eapply Hk2.
+       + simpl. unfold distinct in Hdist'. destruct Hdist'.
+                        unfold distinct_r in H1.
+                        simpl in H1.
+                        repeat (rewrite -> labels_l_cons in H1).
+                        eapply NoDup_app in H1.
+                        eapply NoDup_cons_1_1. destruct H1.
+                        eapply (submseteq_NoDup _ [channel'; getKey'; schannel_r]); [solve_submseteq | apply H1].  }
+     brel_pures.
+       (* set (keytheory := iLblSig_to_iLblThy [([keyleak1], [keyleak2], keyleak keyleak1 keyleak2)]).*)
+     set (keytheory := keyeff).
+     set (leaktheory := autheff).
+        (* set (leaktheory := (iLblSig_to_iLblThy [([leakauth1], [leakauth2], leakauth leakauth1 leakauth2)])).*)
+         set (M := [([leaksec'; schannel_l], [channel'; getKey'; schannel_r], @iThyBot Σ)]).
+         (* set (N := [([channel'; getKey'; schannel_l], [leaksec'; schannel_r], @iThyBot Σ)] ++ keytheory ++ leaktheory ++ (iLblSig_to_iLblThy L)).*)
+         set (N := [([leaksec'; schannel_l], [channel'; getKey'; schannel_r], @iThyBot Σ)] ++
+                     iLblSig_to_iLblThy (sem_row_union keytheory (sem_row_union leaktheory L))).
+         repeat foldkont.
+         brel_pures.
+         set (leftkontbind := ( match: "r" with
+       InjL <> => kont (InjLV #()%V)
+     | InjR "w" =>
+       kysnd_l alice;; 
+       match: ! #l_key with
+         InjL <> => kont (InjLV #()%V)
+       | InjR "key" => kont (InjR "key")
+       end
+     end )%E).
+         set (rightkontbind := ( match: "r" with
+       InjL <> => kont0 (InjLV #()%V)
+     | InjR "x" =>
+       kysnd_r alice;; 
+       match: ! #l_m'sim with
+         InjL <> => kont0 (InjLV #()%V)
+       | InjR "_" =>
+         let: "rla" := arcv_r bob in
+         match: "rla" with
+           InjL <> => kont0 (InjLV #()%V)
+         | InjR "x" => kont0 ! #l_sim
+         end
+       end
+                                 end )%E).
+          iApply (brel_bind'' _ _  (iLblSig_to_iLblThy (keytheory))  [([leaksec'; schannel_l], [channel'; getKey'; schannel_r], @iThyBot Σ)] (([leaksec'; schannel_l], [channel'; getKey'; schannel_r], iThyBot)
+     :: iLblSig_to_iLblThy (sem_row_union leaktheory (sem_row_union keytheory L))) (𝟙%T) (kyrcv_l alice) (kyrcv_r alice)).
+         { simpl. unfold labels_l. simpl. set_solver. }
+        { simpl. unfold labels_r. simpl. set_solver. }
+        { iApply to_iThy_le_intro'. unfold M. unfold N. unfold sem_row_union. repeat (rewrite -> iLblSig_to_iLblThy_proj; rewrite -> iLblSig_to_iLblThy_app). solve_submseteq. }
+        iApply brel_wand.
+          {  iDestruct "Hkeyrcv" as "#Hkeyrcv".
+            iSpecialize ("Hkeyrcv" $! alice alice).
+            iApply "Hkeyrcv". unfold sem_ty_sum, sem_ty_unit.
+            iExists #()%V, #()%V. unfold alice.
+            repeat (iSplit); try (iPureIntro); try reflexivity.
+            right. repeat split; try reflexivity. }
+         iModIntro. iIntros (v1 v2) "#Hv1v2". brel_pures.
+         unfold sem_ty_group, sem_ty_option, sem_ty_sum.
+         iDestruct "Hv1v2" as (?w1 ?w2) "[#Hnone | #Hsome]".
+         (*key receive didnt return successfully*)
+          - iDestruct "Hnone" as "[%Hv1 [%Hv2 #Hw1w2]]".
+            rewrite -> Hv1. rewrite -> Hv2. unfold sem_ty_unit.
+            iDestruct "Hw1w2" as "(%Hw1 & %Hw2)".
+            rewrite -> Hw1. rewrite -> Hw2. brel_pures.
+            iApply (brel_exhaustion (fill k1'(InjLV #()%V)) (fill k2' (InjLV #()%V))).
+            { simpl. auto. }
+            { simpl. set_solver. }
+            { iApply "Hrel". iDestruct "HmQ" as "[Hsome Hnone]". iApply "Hnone".  }
+            { iApply "IH". }
+          (*key receive returned successfully*)
+           - iDestruct "Hsome" as "[%Hv1 [%Hv2 #Hw1w2]]". 
+             rewrite -> Hv1. rewrite -> Hv2.
+             iDestruct "Hw1w2" as "(%Hw1 & %Hw2)".
+             rewrite -> Hw1. rewrite -> Hw2. brel_pures.
+             (*iApply (brel_bind'' _ _ (iLblSig_to_iLblThy keytheory) M N 𝟙%T (kysnd_l alice) (kysnd_r alice)).*) 
+             set (rightapp := ( match: "rla" with
+                                 InjL <> => kont0 (InjLV #()%V)
+                               | InjR "x" => kont0 ! #l_sim
+                                end)%E).
+              iApply (brel_bind'' _ _ (iLblSig_to_iLblThy keytheory)  [([leaksec'; schannel_l], [channel'; getKey'; schannel_r], @iThyBot Σ)] ([([leaksec'; schannel_l], [channel'; getKey'; schannel_r], @iThyBot Σ)] ++
+                     iLblSig_to_iLblThy (sem_row_union leaktheory (sem_row_union keytheory L))) 𝟙%T (kysnd_l alice) (kysnd_r alice)).
+             { simpl. set_solver. }
+             { simpl. set_solver. }
+             { iApply to_iThy_le_intro'. unfold M. unfold N. unfold sem_row_union. repeat (rewrite -> iLblSig_to_iLblThy_proj; rewrite -> iLblSig_to_iLblThy_app). solve_submseteq. } 
+             iApply brel_wand.
+             { iDestruct "Hkeysnd" as "#Hkeysnd".
+               iSpecialize ("Hkeysnd" $! alice alice).
+               iApply "Hkeysnd".
+               iExists #()%V, #()%V. unfold alice.
+               iRight. repeat (iSplit); try (iPureIntro); try reflexivity. }
+             iModIntro. iIntros (v0 v3) "#HRv0v3".
+             unfold R. unfold sem_ty_unit.
+             iDestruct "HRv0v3" as "(%Hv0 & %Hv3)".
+             rewrite -> Hv0. rewrite -> Hv3. brel_pures.
+             repeat foldkont.
+               iApply (brel_na_inv _ _ alphaN); first set_solver. 
+         iFrame "Hinvα".
+         iIntros "([(>Hγ & >Hl_m'sim & >Hl_sim & >Hl_auth & >Hl_fchan & >Hl_rchan & >Hl_key) | [>Hd2 | >Hd3 ]] & Hclose)".
+                  (* no message has been sent yet by the secure channel*)
+                  ++ iApply (brel_load_r _ _ _ _ [CaseCtx _ _] with "Hl_key").
+                     iIntros "Hl_key". brel_pures.
+                     iApply (brel_load_l _ _ _ [CaseCtx _ _] with "Hl_m'sim").
+                     iIntros "!> Hl_m'sim". brel_pures. simpl.
+                     iApply brel_na_close. iFrame.
+                     iSplitL.
+                     { iModIntro. iLeft. iFrame. }
+                     
+                      iApply (brel_exhaustion (fill k1'(InjLV #()%V)) (fill k2' (InjLV #()%V))).
+                               { simpl. auto. }
+                               { simpl. set_solver. }
+                               { iApply "Hrel". iDestruct "HmQ" as "[Hsome Hnone]". iApply "Hnone".  }
+                               { iApply "IH". }
+                               (* a message has been sent by both the secure channel and the authenticated channel *)
+                ++ unfold d2.
+                   iDestruct "Hd2" as (?m ?n) "(Hγ & (Hl_m'sim & (Hl_sim & (Hl_auth & (Hl_fchan & (Hl_rchan & Hl_key))))))".
+                    iApply (brel_load_r _ _ _ _ [CaseCtx _ _] with "Hl_key").
+                    iIntros "Hl_key". brel_pures.
+                    { simpl. set_solver. }
+                     iApply (brel_load_l _ _ _ [CaseCtx _ _] with "Hl_m'sim").
+                    iIntros "!> Hl_m'sim". brel_pures. simpl.
+                    repeat foldkont.
+                    iApply fupd_brel.
+                    iMod (ghost_map_elem_persist with "Hl_fchan") as "#Hl_fchan".
+                    iMod (ghost_map_elem_persist with "Hl_rchan") as "#Hl_rchan".
+                    iMod (ghost_map_elem_persist with "Hl_key") as "#Hl_key".
+                    iMod (ghost_map_elem_persist with "Hl_m'sim") as "#Hl_m'sim".
+                    iMod (ghost_map_elem_persist with "Hl_auth") as "#Hl_auth".
+                    iMod (ghost_map_elem_persist with "Hl_sim") as "#Hl_sim".
+                    iModIntro.
+                    
+                    iApply brel_na_close. iFrame.
+                    iSplitL.
+                    { iModIntro. iRight. iLeft. iFrame "#". }
+                     iApply (brel_bind'' _ _  (iLblSig_to_iLblThy leaktheory)  [([leaksec'; schannel_l], [channel'; getKey'; schannel_r], @iThyBot Σ)] ([([leaksec'; schannel_l], [channel'; getKey'; schannel_r], @iThyBot Σ)] ++
+                                                                                                                                                   iLblSig_to_iLblThy (sem_row_union leaktheory (sem_row_union keytheory L))) 𝟙%T (arcv_l bob) (arcv_r bob)).
+               { simpl. set_solver. }
+               { simpl. set_solver. }
+               { iApply to_iThy_le_intro'. unfold sem_row_union. repeat (rewrite -> iLblSig_to_iLblThy_proj; rewrite -> iLblSig_to_iLblThy_app). solve_submseteq. }
+               
+               iApply brel_wand.
+               { iDestruct "Harcv" as "#Harcv".
+                 iSpecialize ("Harcv" $! bob bob).
+                 iApply "Harcv".
+                 iExists #()%V, #()%V. unfold bob.
+                 iLeft. repeat (iSplit); try (iPureIntro); try reflexivity. }
+               iModIntro. iIntros (v4 v5) "#Hv4v5".
+               iDestruct "Hv4v5" as (?w0 ?w3) "Hv4v5".
+               iDestruct "Hv4v5" as "[Hnone | Hsome]".
+               +++ (* leakauth doesnt return successfully *)
+                 iDestruct "Hnone" as "(%Hv4 & (%Hv5 & (%Hw0 & %Hw3)))".
+                 rewrite -> Hv4. rewrite -> Hv5. rewrite -> Hw0. rewrite -> Hw3.
+                 brel_pures.
+                   iApply (brel_exhaustion (fill k1' (InjLV #()%V)) (fill k2' (InjLV #()%V))).
+                          { simpl. set_solver. }
+                          { simpl. set_solver. }
+                          { iApply "Hrel".  iDestruct "HmQ" as "[Hsome Hnone]". iApply "Hnone". }
+                          {iApply "IH". }
+               +++ (* leakauth returns successfully with a value *)
+                   iDestruct "Hsome" as "(%Hv4 & (%Hv5 & (%Hw0 & %Hw3)))".
+                   rewrite -> Hv4. rewrite -> Hv5. rewrite -> Hw0. rewrite -> Hw3.
+                   brel_pures.
+                              iApply (brel_load_l _ _ _ [AppRCtx _] with "Hl_sim").
+                              iIntros "!> Hl_sim'".
+                              iApply (brel_load_r _ _ _ _ [HandleCtx _ _ _ _ _ ; AppRCtx _] with "Hl_auth").
+                              iIntros "Hl_auth'".
+                              iDestruct "Hl_fchan" as "#Hl_fchan".
+                              simpl. brel_pures.
+                               (*iApply brel_na_close. iFrame.
+                               iSplitL; [iModIntro; iRight; iLeft; iFrame; iFrame "#" |].
+                               brel_pures.*)
+                               iApply G_XOR_CORRECT_r.
+                               { rewrite -> vg_int_xor_sem. repeat (rewrite -> Bij_xor_sem). reflexivity. }
+                               brel_pures.
+                               iApply (brel_load_l _ _ _ [HandleCtx _ _ _ _ _ ; AppRCtx _ ] with "Hl_fchan").
+                               iIntros "!> Hl_fchan'".
+                               brel_pures.
+                                set (g_enc := (group_xor_sem
+                                        (group_xor_sem m (g ^+ f m n))
+                                        (g ^+ f m n))).
+                               iApply (brel_exhaustion (fill k1'((InjRV (vgval m))%V)) (fill k2' ((InjRV (vgval g_enc)))%V)).
+                               { simpl. auto.}
+                                { simpl. set_solver. }
+                               { unfold kont0. iApply "Hrel". iDestruct "HmQ" as "[Hsome Hnone]". unfold g_enc. rewrite -> Bij_xor_sem. iApply "Hsome". }
+                               { iApply "IH". }
+                               (* a message has been sent by the secure channel but not the authenticated channel*)
+                           ++ simpl. brel_pures.
+                              unfold d3.
+                              iDestruct "Hd3" as (?m ?n) "(Hγ & (Hl_m'sim & (Hl_sim & (Hl_auth & (Hl_fchan & (Hl_rchan & Hl_key))))))". 
+                               iApply (brel_load_r _ _ _ _ [CaseCtx _ _] with "Hl_key").
+                               iIntros "Hl_key". brel_pures.
+                               { simpl. set_solver. }
+                               iApply (brel_load_l _ _ _ [CaseCtx _ _] with "Hl_m'sim").
+                               iIntros "!> Hl_m'sim". brel_pures. simpl.
+                               repeat foldkont.
+                               iApply fupd_brel.
+                               iMod (ghost_map_elem_persist with "Hl_fchan") as "#Hl_fchan".
+                               iMod (ghost_map_elem_persist with "Hl_rchan") as "#Hl_rchan".
+                              iMod (ghost_map_elem_persist with "Hl_key") as "#Hl_key".
+                              iMod (ghost_map_elem_persist with "Hl_m'sim") as "#Hl_m'sim".
+                              iModIntro.
+                    
+                       iApply brel_na_close. iFrame.
+                       iSplitL.
+                       { iModIntro. iRight. iRight. iFrame "#". iFrame. }
+           iApply (brel_bind'' _ _  (iLblSig_to_iLblThy leaktheory)  [([leaksec'; schannel_l], [channel'; getKey'; schannel_r], @iThyBot Σ)] ([([leaksec'; schannel_l], [channel'; getKey'; schannel_r], @iThyBot Σ)] ++
+                                                                                                                                                   iLblSig_to_iLblThy (sem_row_union leaktheory (sem_row_union keytheory L))) 𝟙%T (arcv_l bob) (arcv_r bob)).
+               { simpl. set_solver. }
+               { simpl. set_solver. }
+               { iApply to_iThy_le_intro'. unfold sem_row_union. repeat (rewrite -> iLblSig_to_iLblThy_proj; rewrite -> iLblSig_to_iLblThy_app). solve_submseteq. }
+               
+               iApply brel_wand.
+               { iDestruct "Harcv" as "#Harcv".
+                 iSpecialize ("Harcv" $! bob bob).
+                 iApply "Harcv".
+                 iExists #()%V, #()%V. unfold bob.
+                 iLeft. repeat (iSplit); try (iPureIntro); try reflexivity. }
+               iModIntro. iIntros (v4 v5) "#Hv4v5".
+               iDestruct "Hv4v5" as (?w0 ?w3) "Hv4v5".
+               iDestruct "Hv4v5" as "[Hnone | Hsome]".
+               (* leakauth doesnt return successfully *)
+               +++ iDestruct "Hnone" as "(%Hv4 & (%Hv5 & (%Hw0 & %Hw3)))".
+                 rewrite -> Hv4. rewrite -> Hv5. rewrite -> Hw0. rewrite -> Hw3.
+                 brel_pures.
+                   iApply (brel_exhaustion (fill k1' (InjLV #()%V)) (fill k2' (InjLV #()%V))).
+                          { simpl. set_solver. }
+                          { simpl. set_solver. }
+                          { iApply "Hrel".  iDestruct "HmQ" as "[Hsome Hnone]". iApply "Hnone". }
+                          {iApply "IH". }
+              (* leakauth returns successfully with a value *)
+               +++ iDestruct "Hsome" as "(%Hv4 & (%Hv5 & (%Hw0 & %Hw3)))".
+                  rewrite -> Hv4. rewrite -> Hv5. rewrite -> Hw0. rewrite -> Hw3.
+                  brel_pures.
+                           (*another case analysis by opening the invariant again, since we need access to the pointers l_sim and l_auth *)
+                            iApply (brel_na_inv _ _ alphaN); first set_solver. 
+                            iFrame "Hinvα".
+                            iIntros "([(>Hγ & >Hl_m'sim' & >Hl_sim & >Hl_auth & >Hl_fchan' & >Hl_rchan' & >Hl_key') | [>Hd2 | >Hd3 ]] & Hclose)".
+                            (*contradiction branch since we already know that a message has been sent by the secure channel *)
+                           -- iDestruct (ghost_map_elem_agree
+                                        with "Hl_fchan Hl_fchan'") as %Heq.
+                              congruence.
+                            (*the next two brances will move the proof forward with a case analysis on l_auth and l_sim having been set or not *)
+                           -- unfold d2. 
+                              iDestruct "Hd2" as (?m ?n) "(Hγ & (Hl_m'sim' & (Hl_sim & (Hl_auth & (Hl_fchan' & (Hl_rchan' & Hl_key'))))))".
+                              iApply (brel_load_l _ _ _ [AppRCtx _] with "Hl_sim").
+                              iIntros "!> Hl_sim".
+                              iApply (brel_load_r _ _ _ _ [HandleCtx _ _ _ _ _ ; AppRCtx _] with "Hl_auth").
+                              iIntros "Hl_auth".
+                              iApply fupd_brel.
+                              iMod (ghost_map_elem_persist with "Hl_fchan'") as "#Hl_fchan'".
+                              iMod (ghost_map_elem_persist with "Hl_rchan'") as "#Hl_rchan'".
+                              iMod (ghost_map_elem_persist with "Hl_key'") as "#Hl_key'".
+                              iMod (ghost_map_elem_persist with "Hl_m'sim'") as "#Hl_m'sim'".
+                              iMod (ghost_map_elem_persist with "Hl_auth") as "#Hl_auth".
+                              iMod (ghost_map_elem_persist with "Hl_sim") as "#Hl_sim".
+                              iModIntro.
+                    
+                       iApply brel_na_close. iFrame.
+                       iSplitL.
+                       { iModIntro. iRight. iLeft. iFrame "#". }
+                       simpl. brel_pures.
+                       iCombine "Hl_fchan Hl_fchan'" gives %[Hval Hval2].
+                                  inversion Hval2. apply vgval_inj in H1. rewrite -> H1.
+                                  iCombine "Hl_m'sim Hl_m'sim'" gives %[Hsim Hsim2]. clear Hval Hsim.
+                                  inversion Hsim2. specialize (Hf m0). destruct Hf as [Hfinj Hfsurj].
+                                  apply Nat2Z.inj in H2.
+                                  (*apply fin_to_nat_inj in H2.
+                                  apply (@inj _ _ eq eq (f m0) Hfinj n n0) in H2.*)
+                                  rewrite -> H2.
+                               iApply G_XOR_CORRECT_r.
+                               { rewrite -> vg_int_xor_sem. repeat (rewrite -> Bij_xor_sem). reflexivity. }
+                               brel_pures.
+                               iApply (brel_load_l _ _ _ [HandleCtx _ _ _ _ _ ; AppRCtx _ ] with "Hl_fchan").
+                               iIntros "!> Hl_fchan''".
+                               brel_pures.
+                                set (g_enc := (group_xor_sem
+                                        (group_xor_sem m0 (g ^+  f m0 n0))
+                                        (g ^+ f m0 n0))).
+                               iApply (brel_exhaustion (fill k1'((InjRV (vgval m0))%V)) (fill k2' ((InjRV (vgval g_enc)))%V)).
+                               { simpl. auto. }
+                                { simpl. set_solver. }
+                                { unfold kont0. iApply "Hrel". iDestruct "HmQ" as "[Hsome Hnone]".
+                                   unfold g_enc.
+                                  rewrite -> Bij_xor_sem. iApply "Hsome". }
+                               { iApply "IH". }
+                           -- unfold d3.
+                              iDestruct "Hd3" as (?m ?n) "(Hγ & (Hl_m'sim' & (Hl_sim & (Hl_auth & (Hl_fchan' & (Hl_rchan' & Hl_key'))))))".
+                               iApply (brel_load_l _ _ _ [AppRCtx _] with "Hl_sim").
+                              iIntros "!> Hl_sim".
+                              iApply (brel_load_r _ _ _ _ [HandleCtx _ _ _ _ _ ; AppRCtx _] with "Hl_auth").
+                              iIntros "Hl_auth".
+                              iApply fupd_brel.
+                              iMod (ghost_map_elem_persist with "Hl_fchan'") as "#Hl_fchan'".
+                              iMod (ghost_map_elem_persist with "Hl_rchan'") as "#Hl_rchan'".
+                              iMod (ghost_map_elem_persist with "Hl_key'") as "#Hl_key'".
+                              iMod (ghost_map_elem_persist with "Hl_m'sim'") as "#Hl_m'sim'".
+                              iModIntro.
+                    
+                             iApply brel_na_close. iFrame.
+                             iSplitL.
+                             { iModIntro. iRight. iRight. iFrame "#". iFrame. }
+                             simpl. brel_pures.
+                             iApply (brel_exhaustion (fill k1' (InjLV #()%V)) (fill k2' (InjLV #()%V))).
+                            { simpl. set_solver. }
+                            { simpl. set_solver. }
+                            { iApply "Hrel".  iDestruct "HmQ" as "[Hsome Hnone]". iApply "Hnone". }
+                            { iApply "IH". }
+Qed.
 
 
 
@@ -2080,7 +3001,7 @@ Lemma R_CHAN_CHAN_SIM_F_CHAN :
   ⊢ sem_val_typed (R_CHAN)%V (λ: "f", CHAN_SIM_lazy (F_CHAN "f"))%V
       (∀ᵣ θ__L ,(∀ᵣ θₕ, (((𝔾 -{ θₕ }->  𝟙) × (𝟙 -{ θₕ }-> (Option  𝔾))) -{ sem_row_union  θₕ θ__L }-∘ 𝟙)) ⊸ (*type of client*)
       (∀ᵣ θ₁, ∀ᵣ θ₂,  (((𝔾 × (𝟙 + 𝟙)) -{ θ₁ }-> 𝟙) × ((𝟙 + 𝟙) -{ θ₁ }-> Option 𝟙)) ⊸ (((𝟙 + 𝟙) -{ θ₂ }-> 𝟙) × (𝟙 + 𝟙) -{ θ₂ }-> Option 𝟙) -{ sem_row_union θ₁ (sem_row_union θ₂ θ__L) }-∘ 𝟙))%T.
-Proof using Bdd_int_vg Bij_log Bij_xor_sem G H
+Proof using Bdd_int_vg Bij_log Bij_xor_sem Bij_xor_sem_l G H
 Val_log XOR_spec0 cg group_xor_sem inG0 inG1 inG2
 log__g vg vg_int_xor_sem vgg xor_struct Σ.
   iModIntro. iIntros (L).
@@ -2099,7 +3020,10 @@ Lemma CHAN_SIM_F_CHAN_R_CHAN :
    ⊢ sem_val_typed (λ: "f", CHAN_SIM_lazy (F_CHAN "f"))%V (R_CHAN)%V
       (∀ᵣ θ__L ,(∀ᵣ θₕ, (((𝔾 -{ θₕ }->  𝟙) × (𝟙 -{ θₕ }-> (Option  𝔾))) -{ sem_row_union  θₕ θ__L }-∘ 𝟙)) ⊸ (*type of client*)
                 (∀ᵣ θ₁, ∀ᵣ θ₂,  (((𝔾 × (𝟙 + 𝟙)) -{ θ₁ }-> 𝟙) × ((𝟙 + 𝟙) -{ θ₁ }-> Option 𝟙)) ⊸ (((𝟙 + 𝟙) -{ θ₂ }-> 𝟙) × (𝟙 + 𝟙) -{ θ₂ }-> Option 𝟙) -{ sem_row_union θ₁ (sem_row_union θ₂ θ__L) }-∘ 𝟙))%T.
- Proof using G inG0 inG1 inG2.
+ Proof using Bdd_int_vg Bij_log Bij_xor_sem
+Bij_xor_sem_l G H Val_log XOR_spec0 cg
+group_xor_sem inG0 inG1 inG2 log__g vg
+vg_int_xor_sem vgg xor_struct Σ.
   iModIntro. iIntros (L).
   iIntros (f1 f2) "Hrelf1f2".
   brel_pures'.
@@ -2118,7 +3042,7 @@ Lemma R_I_SCHAN :
   ⊢ sem_typed [] R_CHAN (λ: "f", (CHAN_SIM_lazy (F_CHAN "f")))%V ⊥
        (∀ᵣ θ__L ,(∀ᵣ θₕ, (((𝔾 -{ θₕ }-> 𝟙) × (𝟙 -{ θₕ }-> (Option  𝔾))) -{ sem_row_union  θₕ θ__L }-∘ 𝟙)) ⊸ (*type of client*)
                  (∀ᵣ θ₁, ∀ᵣ θ₂,  (((𝔾 × (𝟙 + 𝟙)) -{ θ₁ }-> 𝟙) × ((𝟙 + 𝟙) -{ θ₁ }-> Option 𝟙)) ⊸ (((𝟙 + 𝟙) -{ θ₂ }-> 𝟙) × ((𝟙 + 𝟙) -{ θ₂ }-> Option 𝟙)) -{ sem_row_union θ₁ (sem_row_union θ₂ θ__L) }-∘ 𝟙))%T [].
-Proof using Bdd_int_vg Bij_log Bij_xor_sem G H
+Proof using Bdd_int_vg Bij_log Bij_xor_sem Bij_xor_sem_l G H
 Val_log XOR_spec0 cg group_xor_sem inG0 inG1 inG2
 klk1 klk2 lka1 lka2 log__g vg vg_int_xor_sem vgg
 xor_struct Σ.
@@ -2136,7 +3060,10 @@ Lemma I_R_SCHAN :
  ⊢ sem_typed [] (λ: "f", (CHAN_SIM_lazy (F_CHAN "f")))%V R_CHAN ⊥
        (∀ᵣ θ__L ,(∀ᵣ θₕ, (((𝔾 -{ θₕ }-> 𝟙) × (𝟙 -{ θₕ }-> (Option  𝔾))) -{ sem_row_union  θₕ θ__L }-∘ 𝟙)) ⊸ (*type of client*)
                  (∀ᵣ θ₁, ∀ᵣ θ₂,  (((𝔾 × (𝟙 + 𝟙)) -{ θ₁ }-> 𝟙) × ((𝟙 + 𝟙) -{ θ₁ }-> Option 𝟙)) ⊸ (((𝟙 + 𝟙) -{ θ₂ }-> 𝟙) × ((𝟙 + 𝟙) -{ θ₂ }-> Option 𝟙)) -{ sem_row_union θ₁ (sem_row_union θ₂ θ__L) }-∘ 𝟙))%T [].
-Proof using G inG0 inG1 inG2 klk1 klk2 lka1 lka2.
+Proof using Bdd_int_vg Bij_log Bij_xor_sem
+Bij_xor_sem_l G H Val_log XOR_spec0 cg
+group_xor_sem inG0 inG1 inG2 klk1 klk2 lka1 lka2
+log__g vg vg_int_xor_sem vgg xor_struct Σ. 
   iIntros (vs) "!# H". simpl.
   iApply brel_value.
   iIntros "$ !>".
